src/program_proof/session/gossip.v
@@ -1,0 +1,47 @@
+From Perennial.program_proof.session Require Export session_prelude coq_session.
+From Perennial.program_proof.session Require Export versionVector sort.
+
+
+Section heap.
+
+  Context `{hG: !heapGS Σ}.
+
+  Lemma wp_acknowledgeGossip (sv: u64*u64*Slice.t*Slice.t*Slice.t*Slice.t*Slice.t*Slice.t) (s: Server.t) (msgv: u64*u64*u64*u64*u64*Slice.t*u64*u64*Slice.t*u64*u64*u64*u64*u64*u64*Slice.t*u64*u64) (msg: Message.t) (n: nat) :
+    {{{
+          is_server sv s n ∗ 
+          is_message msgv msg n
+    }}}
+      acknowledgeGossip (server_val sv) (message_val msgv)
+      {{{
+            r , RET r;
+            is_server sv (coq_acknowledgeGossip s msg) n ∗
+            is_message msgv msg n
+      }}}.
+  Proof.
+    iIntros "%Φ (H1 & H2) H_ret".
+    rewrite /acknowledgeGossip.
+    iDestruct "H1" as "(%H1 & %H2 & H1 & %H3 & H4 & H5 & H6 & H7 & %H4 & H8)".
+    iDestruct "H2" as "(%H5 & %H6 & %H7 & %H8 & %H9 & %H10 & H9 & %H11 & %H12 & H10 & %H13 & %H14 & %H15 & %H16 & %H17 & %H18 & %H19 & H11 & %H20 & %H21)".
+    wp_pures.
+    wp_apply (wp_slice_len).
+    wp_if_destruct.
+    { iModIntro. iApply "H_ret". iFrame. admit. }
+    iDestruct (own_slice_small_sz with "H8") as "%H22". 
+    assert (uint.nat msgv.1.1.1.1.1.1.1.2 < length s.(Server.GossipAcknowledgements))%nat
+      by word.
+    apply list_lookup_lt in H as [x H].
+    wp_apply (wp_SliceGet with "[H8]"). { iFrame. auto. }
+    iIntros "H8".
+    wp_apply (wp_maxTwoInts with "[]"). { auto. }
+    iIntros (r) "%H23".
+    wp_pures.
+    rewrite H23.
+    wp_apply (slice.wp_SliceSet with "[H8]"). { iSplitL "H8".
+                                                - iApply "H8".
+                                                - iPureIntro. split; auto. admit. }
+    iIntros "H". wp_pures. iModIntro.
+    iApply "H_ret".
+  Admitted.
+    
+    
+End heap.
